src/BigStep/Coverage.v
@@ -205,12 +205,12 @@ match clock with
                  | None => 
                  let tlf := get_own_modfunc own_module (fst f) (snd f) ( modules ++ stdlib) in
                  match tlf with
-                   | Some func  => (Result id (inl [VClos env [] id (varl func) (body func)]) eff, log_increase (inl _EVAL_FUNID_MODULE) log)
+                   | Some func  => (Result id (inl [VClos env [] id (varl func) (body func) None]) eff, log_increase (inl _EVAL_FUNID_MODULE) log)
                    | None => (Failure, log)
                  end
               end
 
-   | EFun vl e => (Result (S id) (inl [VClos env [] id vl e]) eff, log_increase (inl _EVAL_FUN) log)
+   | EFun vl e => (Result (S id) (inl [VClos env [] id vl e None]) eff, log_increase (inl _EVAL_FUN) log)
    | ECons hd tl => 
      match fbs_expr clock' log env modules own_module id tl eff with
        | (Result id' (inl [tlv]) eff', log') =>
@@ -273,7 +273,7 @@ match clock with
          match res with
          | (Result id'' (inl vl) eff'', log'') => 
            match v with
-           | VClos ref ext closid varl body =>
+           | VClos ref ext closid varl body fid =>
               if Nat.eqb (length varl) (length vl)
               then fbs_expr clock' (log_increase (inl _EVAL_APP) log'') (append_vars_to_env varl vl (get_env ref ext)) modules own_module id'' body eff''
               else (Result id'' (inr (badarity v)) eff'', log_increase (inl _EVAL_APP_EX_BADARITY) log'')
