src/BigStep/Environment.v
@@ -9,7 +9,7 @@ Definition Environment : Type := list ((Var + FunctionIdentifier) * Value).
 Fixpoint count_closures (env : Environment) : nat :=
 match env with
 | [] => 0
-| (_, VClos _ _ _ _ _)::xs => S (count_closures xs)
+| (_, VClos _ _ _ _ _ _)::xs => S (count_closures xs)
 | _::xs => count_closures xs
 end.
 
@@ -90,7 +90,7 @@ match vl, paramss, bodies with
 | [], [], [] => d
 | v::vs, varl::ps, e::bs => append_funs_to_env_base vs ps bs 
                               (insert_value d (inr v) 
-                                           (VClos def deffuns last_id varl e)) 
+                                           (VClos def deffuns last_id varl e (Some v))) 
                                            def deffuns (S last_id)
 | _, _, _ => []
 end.
@@ -116,11 +116,11 @@ Goal append_funs_to_env [(("f1"%string,0), ([], ErrorExp)) ;
        (inr ("f1"%string, 0),
        VClos [(inl "X"%string, VLit (Atom "error"))]
          [(2, ("f1"%string, 0), ([], ELit (Atom "error")));
-         (1, ("f2"%string, 0), ([], ELit (Atom "error")))] 2 [] (ELit (Atom "error")));
+         (1, ("f2"%string, 0), ([], ELit (Atom "error")))] 2 [] (ELit (Atom "error")) (Some ("f1"%string, 0)));
        (inr ("f2"%string, 0),
        VClos [(inl "X"%string, VLit (Atom "error"))]
          [(2, ("f1"%string, 0), ([], ELit (Atom "error")));
-         (1, ("f2"%string, 0), ([], ELit (Atom "error")))] 1 [] (ELit (Atom "error")))].
+         (1, ("f2"%string, 0), ([], ELit (Atom "error")))] 1 [] (ELit (Atom "error")) (Some ("f2"%string, 0)))].
 Proof. reflexivity. Qed.
 Goal insert_function 2 ("f1"%string, 0) [] ErrorExp (list_functions
                               [("f1"%string,0); ("f2"%string,0); ("f1"%string, 0)]
@@ -136,7 +136,7 @@ Fixpoint get_env_base (env def : Environment)
    : Environment :=
 match ext with
 | [] => env
-| (id, f1, (pl, b))::xs => get_env_base (insert_value env (inr f1) (VClos def defext id pl b)) def xs defext
+| (id, f1, (pl, b))::xs => get_env_base (insert_value env (inr f1) (VClos def defext id pl b None)) def xs defext
 end.
 
 Definition get_env (env : Environment) 
