src/TMP/Task/Equivalence.v
@@ -1,5 +1,6 @@
 From CoreErlang.BigStep Require Import BigStep.
 Require Import Coq.Lists.List.
+Require Import stdpp.list.
 
 
 Module subst_bigstepigStep.
@@ -11,6 +12,8 @@ Import ListNotations.
 
 Search ((_ -> option _) -> _ -> _ option).
 Search "map".
+Search "mapM".
+Check mapM.
 (*Needed: {A B : Type} (f : A -> option B) (l : list A) : option (list B)*)
 
 Fixpoint sequence {A : Type} (l : list (option A)) : option (list A) :=
@@ -30,32 +33,30 @@ Fixpoint value_to_expression (v : Value) : option Expression :=
   | VNil => Some ENil
   | VLit l => Some (ELit l)
   (*TODO*)
-  | VClos env ext id vl e => None(*match (subst_bigstep (EFun vl e) env) with
+  | VClos env ext id vl e fid => match (subst_bigstep (EFun vl e) env) with
                               | Some e' => Some (EFun vl e')
                               | None => None
-                              end*)
+                              end
   | VCons hd tl => match (value_to_expression hd), (value_to_expression tl) with
                   | Some hd', Some tl' => Some (ECons hd' tl')
                   | _, _ => None
                   end
-  | VTuple l => match (sequence (map value_to_expression l)) with
+  | VTuple l => match (mapM value_to_expression l) with
                 | Some l' => Some (ETuple  l')
                 | None => None
                 end
-  | VMap l =>  match (sequence (map (fun '(x, y) => match (value_to_expression x), (value_to_expression y) with
+  | VMap l =>  match (mapM (fun '(x, y) => match (value_to_expression x), (value_to_expression y) with
                                                     | Some x', Some y' => Some (x', y')
                                                     | _, _ => None
                                                     end
-                                                    ) l)) with
+                                                    ) l) with
               | Some l' => Some (EMap l')
               | None => None
               end
   end.
-
-
 (*with*) Fixpoint subst_bigstep (e : Expression) (Γ : Environment) : option Expression :=
 match e with
-  | EValues el => match (sequence (map (fun x => subst_bigstep x Γ) el)) with
+  | EValues el => match (mapM (fun x => subst_bigstep x Γ) el) with
                   | Some el' => Some (EValues el')
                   | None => None
                   end
@@ -77,29 +78,29 @@ match e with
                   | Some hd', Some tl' => Some (ECons hd' tl')
                   | _, _ => None
                   end
-  | ETuple l => match (sequence (map (fun x => subst_bigstep x Γ) l)) with
+  | ETuple l => match (mapM (fun x => subst_bigstep x Γ) l) with
                 | Some l' => Some (ETuple l')
                 | None => None
                 end
-  | ECall m f l => match (subst_bigstep m Γ), (subst_bigstep f Γ), (sequence (map (fun x => subst_bigstep x Γ) l)) with
+  | ECall m f l => match (subst_bigstep m Γ), (subst_bigstep f Γ), (mapM (fun x => subst_bigstep x Γ) l)) with
                   | Some m', Some f', Some l' => Some (ECall m' f' l')
                   | _, _, _ => None
                   end
-  | EPrimOp f l => match (sequence (map (fun x => subst_bigstep x Γ) l)) with
+  | EPrimOp f l => match (mapM (fun x => subst_bigstep x Γ) l) with
                   | Some l' => Some (EPrimOp f l')
                   | None => None
                   end
-  | EApp exp l => match (subst_bigstep exp Γ), (sequence (map (fun x => subst_bigstep x Γ) l)) with
+  | EApp exp l => match (subst_bigstep exp Γ), (mapM (fun x => subst_bigstep x Γ) l) with
                   | Some exp', Some l' => Some (EApp exp' l')
                   | _, _ => None
                   end
   | ECase e l => match (subst_bigstep e Γ) with
-                | Some e' => match (sequence (map (fun '(pl, g, b) =>
+                | Some e' => match (mapM (fun '(pl, g, b) =>
                                       match (subst_bigstep g Γ), (subst_bigstep b Γ) with
                                       | Some g', Some b' => Some (pl, g', b')
                                       | _, _ => None
                                       end
-                                    ) l)) with
+                                    ) l) with
                             | Some l' => Some (ECase e' l')
                             | None => None
                             end
@@ -113,20 +114,20 @@ match e with
                   | Some e1', Some e2' => Some (ESeq e1' e2')
                   | _, _ => None
                   end
-  | ELetRec l e => match (sequence (map (fun '(fid, (vl, b)) =>
+  | ELetRec l e => match (mapM (fun '(fid, (vl, b)) =>
                                       match (subst_bigstep b Γ) with
                                       | Some b' => Some (fid, (vl, b'))
                                       | None => None
                                       end
-                                    ) l)), (subst_bigstep e Γ) with
+                                    ) l), (subst_bigstep e Γ) with
                     | Some l', Some e' => Some (ELetRec l' e')
                     | _, _ => None
                     end
-  | EMap l => match (sequence (map (fun '(x, y) => match (subst_bigstep x Γ), (subst_bigstep y Γ) with
+  | EMap l => match (mapM (fun '(x, y) => match (subst_bigstep x Γ), (subst_bigstep y Γ) with
                                                   | Some x', Some y' => Some (x', y')
                                                   | _, _ => None
                                                   end
-                                                  ) l)) with
+                                                  ) l) with
               | Some l' => Some (EMap l')
               | None => None
               end
